Get reflect_and_reverse working and fix build

pulse/examples/steel/AggregateRefExamples.fst
@@ -1,17 +1,14 @@
 module AggregateRefExamples
 
-open Aggregates
 open AggregateRef
-open FStar.PCM
-open FStar.FunctionalExtensionality
 
 open Steel.Effect
 module A = Steel.Effect.Atomic
 
 /// Example 1: swapping the coordinates of a 2d point
 
-open PointStruct
 open PCM.POD
+open PointStruct
 
 /// We can write the following function that swaps the x and y fields of a given point:
 /// 
@@ -40,8 +37,7 @@ let point_swap (p: ref 'a point{p.q == point_pcm}) (x y: Ghost.erased int)
   ref_write r tmp;
   (* Gather *)
   un_addr_of_x p q;
-  un_addr_of_y p r;
-  A.change_equal_slprop (p `pts_to` _) (p `pts_to` _)
+  un_addr_of_y p r
 
 /// We can also implement swap generically:
 ///
@@ -64,8 +60,8 @@ let generic_swap
   ref_write p vy;
   (* *q = tmp *)
   ref_write q tmp;
-  A.change_equal_slprop (p `pts_to` _) (p `pts_to` _);
-  A.change_equal_slprop (q `pts_to` _) (q `pts_to` _)
+  A.change_equal_slprop (p `pts_to` _) (p `pts_to` _)
+  // seems can't get rid of final change_equal_slprop, even with smt_fallback
 
 /// Now, point_swap written using generic_swap:
 ///
@@ -89,113 +85,7 @@ let point_swap_generically
   generic_swap q r;
   (* Gather *)
   un_addr_of_x p q;
-  un_addr_of_y p r;
-  A.change_equal_slprop (p `pts_to` _) (p `pts_to` _)
-
-(*
-/// Example 2: pointers to nested fields
-///
-/// Here's a struct representing a line segment by its two endpoints:
-///   struct line { struct point p1; struct point p2; };
-///
-/// Carrier of PCM for line:
-
-type line_field = | P1 | P2
-let line_fields k = match k with
-  | P1 -> point
-  | P2 -> point
-let line = restricted_t line_field line_fields
-
-/// PCM for line:
-
-let line_fields_pcm k : pcm (line_fields k) = match k with
-  | P1 -> point_pcm
-  | P2 -> point_pcm
-let line_pcm = prod_pcm line_fields_pcm
-
-/// (mk_line p1 p2) represents (struct line){.p1 = p1, .p2 = p2}
-
-let mk_line_f (p1 p2: point) (k: line_field): line_fields k = match k with
-  | P1 -> p1
-  | P2 -> p2
-let mk_line (p1 p2: point): line = on_domain line_field (mk_line_f p1 p2)
-
-/// Laws about putting/getting the x and y fields of a (mk_line x y)
-
-let put_p1 p1' p1 p2
-: Lemma (feq (put (field line_fields_pcm P1) p1' (mk_line p1 p2)) (mk_line p1' p2))
-  [SMTPat (put (field line_fields_pcm P1) p1' (mk_line p1 p2))]
-= ()
-
-let get_p1 p1 p2
-: Lemma (get (field line_fields_pcm P1) (mk_line p1 p2) == p1)
-  [SMTPat (get (field line_fields_pcm P1) (mk_line p1 p2))]
-= ()
-
-let put_p2 p2' p1 p2
-: Lemma (feq (put (field line_fields_pcm P2) p2' (mk_line p1 p2)) (mk_line p1 p2'))
-  [SMTPat (put (field line_fields_pcm P2) p2' (mk_line p1 p2))]
-= ()
-
-let get_p2 p1 p2
-: Lemma (get (field line_fields_pcm P2) (mk_line p1 p2) == p2)
-  [SMTPat (get (field line_fields_pcm P2) (mk_line p1 p2))]
-= ()
-
-/// Laws relating mk_line to PCM operations
-
-let one_line : squash (feq (one line_pcm) (mk_line (one point_pcm) (one point_pcm)))
-= ()
-
-let merge_line p1 p2 p1' p2'
-: Lemma (feq (op line_pcm (mk_line p1 p2) (mk_line p1' p2'))
-             (mk_line (op (line_fields_pcm P1) p1 p1') (op (line_fields_pcm P2) p2 p2')))
-  [SMTPat (op line_pcm (mk_line p1 p2) (mk_line p1' p2'))]
-= ()
-
-/// Taking pointers to the p1 and p2 fields of a line
-
-let addr_of_p1 (p: ref 'a line{p.q == line_pcm}) (p1 p2: Ghost.erased point)
-: SteelT (q:ref 'a point{q == ref_focus p point_pcm (field line_fields_pcm P1)})
-    (p `pts_to` mk_line p1 p2)
-    (fun q ->
-       (p `pts_to` mk_line (one point_pcm) p2) `star`
-       (q `pts_to` p1))
-= let q = addr_of_lens p (field line_fields_pcm P1) (mk_line p1 p2) in
-  A.change_equal_slprop (p `pts_to` _) (p `pts_to` mk_line (one point_pcm) p2);
-  A.change_equal_slprop (q `pts_to` _) (q `pts_to` p1);
-  A.return q
-
-let un_addr_of_p1
-  (p: ref 'a line{p.q == line_pcm})
-  (q: ref 'a point{q == ref_focus p point_pcm (field line_fields_pcm P1)})
-  (p1 p2: Ghost.erased point)
-: SteelT unit
-    ((p `pts_to` mk_line (one point_pcm) p2) `star` (q `pts_to` p1))
-    (fun q -> p `pts_to` mk_line p1 p2)
-= un_addr_of_lens q p (field line_fields_pcm P1) (mk_line (one point_pcm) p2) p1;
-  A.change_equal_slprop (p `pts_to` _) (p `pts_to` _)
-
-let addr_of_p2 (p: ref 'a line{p.q == line_pcm}) (p1 p2: Ghost.erased point)
-: SteelT (q:ref 'a point{q == ref_focus p point_pcm (field line_fields_pcm P2)})
-    (p `pts_to` mk_line p1 p2)
-    (fun q ->
-       (p `pts_to` mk_line p1 (one point_pcm)) `star`
-       (q `pts_to` p2))
-= let q = addr_of_lens p (field line_fields_pcm P2) (mk_line p1 p2) in
-  A.change_equal_slprop (p `pts_to` _) (p `pts_to` mk_line p1 (one point_pcm));
-  A.change_equal_slprop (q `pts_to` _) (q `pts_to` p2);
-  A.return q
-
-let un_addr_of_p2
-  (p: ref 'a line{p.q == line_pcm})
-  (q: ref 'a point{q == ref_focus p point_pcm (field line_fields_pcm P2)})
-  (p1 p2: Ghost.erased point)
-: SteelT unit
-    ((p `pts_to` mk_line p1 (one point_pcm)) `star` (q `pts_to` p2))
-    (fun q -> p `pts_to` mk_line p1 p2)
-= un_addr_of_lens q p (field line_fields_pcm P2) (mk_line p1 (one point_pcm)) p2;
-  A.change_equal_slprop (p `pts_to` _) (p `pts_to` _)
+  un_addr_of_y p r
 
 /// Reflect a line segment across the line y=x and reverse its direction
 ///
@@ -204,73 +94,32 @@ let un_addr_of_p2
 ///   generic_swap(&p.p1.y, &p.p2.x);
 /// }
 
-#push-options "--z3rlimit 20"
+open LineStruct
+
 let reflect_and_reverse
   (p: ref 'a line{p.q == line_pcm}) (x1 y1 x2 y2: Ghost.erased int)
 : SteelT unit
-    (p `pts_to`
-      mk_line
-        (mk_point (some (Ghost.reveal x1)) (some (Ghost.reveal y1)))
-        (mk_point (some (Ghost.reveal x2)) (some (Ghost.reveal y2))))
-    (fun _ ->
-      p `pts_to`
-        mk_line
-          (mk_point (some (Ghost.reveal y2)) (some (Ghost.reveal x2)))
-          (mk_point (some (Ghost.reveal y1)) (some (Ghost.reveal x1))))
-= (* Take all the requisite pointers *)
-  A.change_equal_slprop (p `pts_to` _) (p `pts_to` _);
-  let pp1 =
-    addr_of_p1 p
-      (mk_point (some (Ghost.reveal x1)) (some (Ghost.reveal y1)))
-      (mk_point (some (Ghost.reveal x2)) (some (Ghost.reveal y2)))
-  in
-  A.change_equal_slprop (p `pts_to` _) (p `pts_to` _);
-  let pp2 =
-    addr_of_p2 p
-      (one point_pcm)
-      (mk_point (some (Ghost.reveal x2)) (some (Ghost.reveal y2)))
-  in
-  (* &p.p1.x *)
-  A.change_equal_slprop (pp1 `pts_to` _) (pp1 `pts_to` _);
-  let pp1x = addr_of_x pp1 (some (Ghost.reveal x1)) (some (Ghost.reveal y1)) in
-  (* &p.p1.y *)
-  A.change_equal_slprop (pp1 `pts_to` _) (pp1 `pts_to` _);
-  let pp1y = addr_of_y pp1 none (some (Ghost.reveal y1)) in
-  (* &p.p2.x *)
-  A.change_equal_slprop (pp2 `pts_to` _) (pp2 `pts_to` _);
-  let pp2x = addr_of_x pp2 (some (Ghost.reveal x2)) (some (Ghost.reveal y2)) in
-  (* &p.p2.y *)
-  A.change_equal_slprop (pp2 `pts_to` _) (pp2 `pts_to` _);
-  let pp2y = addr_of_y pp2 none (some (Ghost.reveal y2)) in
-  (* generic_swap(&p.p1.x, &p.p2.y); *)
-  generic_swap pp1x pp2y x1 y2;
+    (p `pts_to` mk_line (mk_point (some x1) (some y1)) (mk_point (some x2) (some y2)))
+    (fun _ -> p `pts_to` mk_line (mk_point (some y2) (some x2)) (mk_point (some y1) (some x1)))
+= (* generic_swap(&p.p1.x, &p.p2.y); *)
+  let pp1 = addr_of_p1 p in
+  let pp1x = addr_of_x pp1 in
+  let pp2 = addr_of_p2 p in
+  let pp2y = addr_of_y pp2 in
+  generic_swap pp1x pp2y;
   (* generic_swap(&p.p1.y, &p.p2.x); *)
-  generic_swap pp1y pp2x y1 x2;
+  let pp1y = addr_of_y pp1 in
+  let pp2x = addr_of_x pp2 in
+  generic_swap pp1y pp2x;
   (* Gather p1 *)
-  A.change_equal_slprop (pp1x `pts_to` _) (pp1x `pts_to` _);
-  A.change_equal_slprop (pp1 `pts_to` _) (pp1 `pts_to` _);
-  un_addr_of_x pp1 pp1x (some (Ghost.reveal y2)) none;
-  A.change_equal_slprop (pp1y `pts_to` _) (pp1y `pts_to` _);
-  A.change_equal_slprop (pp1 `pts_to` _) (pp1 `pts_to` _);
-  un_addr_of_y pp1 pp1y (some (Ghost.reveal y2)) (some (Ghost.reveal x2));
+  un_addr_of_x pp1 pp1x;
+  un_addr_of_y pp1 pp1y;
   (* Gather p2 *)
-  A.change_equal_slprop (pp2x `pts_to` _) (pp2x `pts_to` _);
-  A.change_equal_slprop (pp2 `pts_to` _) (pp2 `pts_to` _);
-  un_addr_of_x pp2 pp2x (some (Ghost.reveal y1)) none;
-  A.change_equal_slprop (pp2y `pts_to` _) (pp2y `pts_to` _);
-  A.change_equal_slprop (pp2 `pts_to` _) (pp2 `pts_to` _);
-  un_addr_of_y pp2 pp2y (some (Ghost.reveal y1)) (some (Ghost.reveal x1));
+  un_addr_of_x pp2 pp2x;
+  un_addr_of_y pp2 pp2y;
   (* Gather p *)
-  A.change_equal_slprop (pp1 `pts_to` _) (pp1 `pts_to` _);
-  A.change_equal_slprop (p `pts_to` _) (p `pts_to` _);
-  un_addr_of_p1 p pp1 (mk_point (some (Ghost.reveal y2)) (some (Ghost.reveal x2))) (one point_pcm);
-  A.change_equal_slprop (pp2 `pts_to` _) (pp2 `pts_to` _);
-  A.change_equal_slprop (p `pts_to` _) (p `pts_to` _);
+  un_addr_of_p1 p pp1;
   un_addr_of_p2 p pp2
-    (mk_point (some (Ghost.reveal y2)) (some (Ghost.reveal x2)))
-    (mk_point (some (Ghost.reveal y1)) (some (Ghost.reveal x1)));
-  A.change_equal_slprop (p `pts_to` _) (p `pts_to` _)
-#pop-options
 
 (*
 addr_of
@@ -281,69 +130,6 @@ addr_of
   (r `pts_to` xs `star` s `pts_to` y)
   (r `pts_to` xs [k `mapsto` y])
   *)
-
-(*
-
-  A.change_equal_slprop (pp1x `pts_to` _) (pp1x `pts_to` _);
-  A.change_equal_slprop (pp1y `pts_to` _) (pp1y `pts_to` _);
-  unfocus pp1x pp1 (field point_fields_pcm X) (some (Ghost.reveal y2));
-  unfocus pp1y pp1 (field point_fields_pcm Y) (some (Ghost.reveal x2));
-  A.change_equal_slprop
-    (pp1 `pts_to` put (field point_fields_pcm X) _ _)
-    (pp1 `pts_to` mk_point (some (Ghost.reveal y2)) none);
-  A.change_equal_slprop
-    (pp1 `pts_to` put (field point_fields_pcm Y) _ _)
-    (pp1 `pts_to` mk_point none (some (Ghost.reveal x2)));
-  gather pp1 (mk_point (some (Ghost.reveal y2)) none) (mk_point none (some (Ghost.reveal x2)));
-  gather pp1 (mk_point (Ghost.reveal (Ghost.hide none)) none) _;
-  (* Gather p2 *)
-  A.change_equal_slprop (pp2x `pts_to` _) (pp2x `pts_to` _);
-  A.change_equal_slprop (pp2y `pts_to` _) (pp2y `pts_to` _);
-  unfocus pp2x pp2 (field point_fields_pcm X) (some (Ghost.reveal y1));
-  unfocus pp2y pp2 (field point_fields_pcm Y) (some (Ghost.reveal x1));
-  A.change_equal_slprop
-    (pp2 `pts_to` put (field point_fields_pcm X) _ _)
-    (pp2 `pts_to` mk_point (some (Ghost.reveal y1)) none);
-  A.change_equal_slprop
-    (pp2 `pts_to` put (field point_fields_pcm Y) _ _)
-    (pp2 `pts_to` mk_point none (some (Ghost.reveal x1)));
-  gather pp2 (mk_point (some (Ghost.reveal y1)) none) (mk_point none (some (Ghost.reveal x1)));
-  gather pp2 (mk_point (Ghost.reveal (Ghost.hide none)) none) _;
-  (* Gather p *)
-  A.change_equal_slprop (pp1 `pts_to` _) (pp1 `pts_to` _);
-  A.change_equal_slprop (pp2 `pts_to` _) (pp2 `pts_to` _);
-  unfocus pp1 p (field line_fields_pcm P1)
-    (mk_point (some (Ghost.reveal y2)) (some (Ghost.reveal x2)));
-  unfocus pp2 p (field line_fields_pcm P2)
-    (mk_point (some (Ghost.reveal y1)) (some (Ghost.reveal x1)));
-  A.change_equal_slprop
-    (p `pts_to` put (field line_fields_pcm P1) _ _)
-    (p `pts_to`
-      mk_line
-        (mk_point (some (Ghost.reveal y2)) (some (Ghost.reveal x2)))
-        (one point_pcm));
-  A.change_equal_slprop
-    (p `pts_to` put (field line_fields_pcm P2) _ _)
-    (p `pts_to`
-      mk_line
-        (one point_pcm)
-        (mk_point (some (Ghost.reveal y1)) (some (Ghost.reveal x1))));
-  gather p
-    (mk_line
-      (mk_point (some (Ghost.reveal y2)) (some (Ghost.reveal x2)))
-      (one point_pcm))
-    (mk_line
-       (one point_pcm)
-       (mk_point (some (Ghost.reveal y1)) (some (Ghost.reveal x1))));
-  gather p (mk_line (Ghost.reveal (Ghost.hide (one point_pcm))) (one point_pcm)) _;
-  //A.change_equal_slprop (pp2 `pts_to` _) _;
-  (* int *r = &p.p1.y; *)
-  (* int *s = &p.p2.x; *)
-  (* int *t = &p.p2.y; *)
-  A.sladmit();
-  A.return ()
-#pop-options
-*)
 
 (*
 pts_to r x
@@ -371,79 +157,6 @@ let f unit : Steel unit fake (fun _ -> _)
 *)
 
 (*
-// let gather (r: ref 'a 'c) (x y: Ghost.erased 'c)
-// : SteelT (_:unit{composable r.q x y})
-//     (to_vprop (r `pts_to` x) `star` to_vprop (r `pts_to` y))
-//     (fun _ -> to_vprop (r `pts_to` op r.q x y))
-
-  (*
-    (to_vprop (r `pts_to` x))
-    (fun _ -> to_vprop (r' `pts_to` put l x (one r'.q)))
-    (fun _ -> r == ref_focus r' q l)
-    (fun _ _ _ -> True)
-    *)
-
-let unfocus #inames (r: ref 'a 'c) (r': ref 'a 'b) (q: refined_one_pcm 'c)
-  (l: pcm_lens r'.q q) (x: Ghost.erased 'c)
-: A.SteelGhost unit inames
-    (to_vprop (r `pts_to` x))
-    (fun _ -> to_vprop (r' `pts_to` put l x (one r'.q)))
-    (fun _ -> r == ref_focus r' q l)
-    (fun _ _ _ -> True)
-= A.change_slprop_rel  
-    (to_vprop (r `pts_to` x))
-    (to_vprop (r' `pts_to` put l x (one r'.q)))
-    (fun _ _ -> True)
-    (fun m -> r'.pl.get_morphism.f_one ())
-*)
-
-(*
-let swap (p: ref 'a point{p.q == point_pcm}) (xy: Ghost.erased int)
-: SteelT unit
-    (to_vprop (p `pts_to` xy))
-    (fun _ -> to_vprop (p `pts_to` mk_point (xy Y) (xy X)))
-  
-let swap (p: ref 'a point{p.q == point_pcm}) (xy: Ghost.erased int)
-: SteelT unit
-    (to_vprop (p `pts_to` xy))
-    (fun _ -> to_vprop (p `pts_to` xy `upd` (X, xy Y) `upd` (Y, xy X)))
-
-let swap (p: ref 'a point{p.q == point_pcm}) (x y: Ghost.erased int)
-: SteelT unit
-    (to_vprop (p `pts_to` mk_point (some (Ghost.reveal x)) (some (Ghost.reveal y))))
-    (fun _ -> to_vprop (p `pts_to` mk_point (some (Ghost.reveal y)) (some (Ghost.reveal x))))
-= let q =
-    addr_of_lens p int_pcm (field point_fields_pcm X)
-      (mk_point (some (Ghost.reveal x)) (some (Ghost.reveal y))) in
-  A.slassert (
-    to_vprop (p `pts_to` mk_point none (some (Ghost.reveal y))) `star`
-    to_vprop (q `pts_to` some (Ghost.reveal x)));
-  A.sladmit ();
-  A.return ()
-*)
-
-// let addr_of_lens (r: ref 'a 'b) (q: refined_one_pcm 'c) (l: pcm_lens r.q q) (x: Ghost.erased 'b)
-// : SteelT (ref 'a 'c)
-//     (to_vprop (r `pts_to` x))
-//     (fun s ->
-//       to_vprop (r `pts_to` put l (one q) x) `star` 
-//       to_vprop (s `pts_to` get l x))
-// = peel r q l x;
-//   focus r q l (put l (get l x) (one r.q)) (get l x)
-
-(*
-let swap (p: ref 'a point) (x y: Ghost.erased (option int))
-: Steel unit
-    (to_vprop (r `pts_to` mk_point x y))
-    (fun _ -> to_vprop (r `pts_to` mk_point y x))
-= 
-let ref_read (r: ref 'a 'b) (x: Ghost.erased 'b)
-: Steel 'b
-    (to_vprop (r `pts_to` x)) 
-    (fun _ -> to_vprop (r `pts_to` x))
-    (requires fun _ -> True)
-    (ensures fun _ x' _ -> compatible r.q x x')*)
-
 (** Example: a model for a tagged union representing colors in RGB or HSV
       type color =
         | RGB : r:int -> g:int -> b:int -> color
@@ -498,5 +211,4 @@ let color_pcm_cases k : pcm (color_cases k) = match k with
   | RGB -> rgb_pcm
   | HSV -> hsv_pcm
 let color_pcm : pcm color_t = union_pcm color_pcm_cases
-
 *)
