pulse/examples/steel/LineStruct.fsti
@@ -1,0 +1,59 @@
+module LineStruct
+
+open Aggregates
+open AggregateRef
+open FStar.PCM
+open Steel.Effect
+open PointStruct
+
+/// Example 2: pointers to nested fields
+///
+/// Here's a struct representing a line segment by its two endpoints:
+///   struct line { struct point p1; struct point p2; };
+///
+/// Carrier of PCM for line:
+
+val line : Type0
+
+/// PCM for line:
+
+val line_pcm : refined_one_pcm line
+
+/// (mk_line p1 p2) represents (struct line){.p1 = p1, .p2 = p2}
+
+val mk_line (x y: Ghost.erased point): Ghost.erased line
+
+/// Lenses for fields
+
+val _p1 : pcm_lens line_pcm point_pcm
+val _p2 : pcm_lens line_pcm point_pcm
+
+/// Taking pointers to the p1 and p2 fields of a line
+
+val addr_of_p1 (#p1 #p2: Ghost.erased point) (p: ref 'a line{p.q == line_pcm})
+: SteelT (q:ref 'a point{q == ref_focus p point_pcm _p1})
+    (p `pts_to` mk_line p1 p2)
+    (fun q ->
+       (p `pts_to` mk_line (one point_pcm) p2) `star`
+       (q `pts_to` p1))
+
+val un_addr_of_p1 (#p1 #p2: Ghost.erased point)
+  (p: ref 'a line{p.q == line_pcm})
+  (q: ref 'a point{q == ref_focus p point_pcm _p1})
+: SteelT unit
+    ((p `pts_to` mk_line (one point_pcm) p2) `star` (q `pts_to` p1))
+    (fun q -> p `pts_to` mk_line p1 p2)
+
+val addr_of_p2 (#p1 #p2: Ghost.erased point) (p: ref 'a line{p.q == line_pcm})
+: SteelT (q:ref 'a point{q == ref_focus p point_pcm _p2})
+    (p `pts_to` mk_line p1 p2)
+    (fun q ->
+       (p `pts_to` mk_line p1 (one point_pcm)) `star`
+       (q `pts_to` p2))
+
+val un_addr_of_p2 (#p1 #p2: Ghost.erased point)
+  (p: ref 'a line{p.q == line_pcm})
+  (q: ref 'a point{q == ref_focus p point_pcm _p2})
+: SteelT unit
+    ((p `pts_to` mk_line p1 (one point_pcm)) `star` (q `pts_to` p2))
+    (fun q -> p `pts_to` mk_line p1 p2)
